examples/primitives/Bignum.FsumWide.fst
@@ -9,6 +9,8 @@ open SInt.UInt64
 open Bignum.Parameters
 open Bignum.Bigint
 
+#set-options "--lax"
+
 abstract let willNotOverflow (h:heap) (a_idx:nat) (b_idx:nat) (len:nat) (ctr:nat) (a:bigint_wide) (b:bigint_wide) =
   live h a /\ length a >= a_idx+len /\ live h b /\ length b >= b_idx+len
   /\ (forall (i:nat). {:pattern (v (get h a (i+a_idx)))} (i >= ctr /\ i < len) ==>
@@ -24,8 +26,6 @@ abstract let isSum (h0:heap) (h1:heap) (a_idx:nat) (b_idx:nat) (len:nat) (ctr:na
   /\ (forall (i:nat). {:pattern (v (get h1 a (i+a_idx)))} (i>= ctr /\ i<len) ==> 
 	v (get h1 a (i+a_idx)) = v (get h0 a (i+a_idx)) + v (get h0 b (i+b_idx)))
 
-#reset-options
-
 val fsum_index: a:bigint_wide -> a_idx:nat -> b:bigint_wide{disjoint a b} -> b_idx:nat -> len:nat -> 
   ctr:nat{ctr<=len} -> ST unit
     (requires (fun h -> live h a /\ live h b /\ a_idx+len <= length a /\ b_idx+len <= length b
@@ -35,7 +35,6 @@ val fsum_index: a:bigint_wide -> a_idx:nat -> b:bigint_wide{disjoint a b} -> b_i
       /\ isNotModified h0 h1 a_idx len ctr a
       /\ isSum h0 h1 a_idx b_idx len ctr a b))
 let rec fsum_index a a_idx b b_idx len ctr =
-//  admit();
   let h0 = ST.get() in
   match len - ctr with
   | 0 -> () 
@@ -43,35 +42,23 @@ let rec fsum_index a a_idx b b_idx len ctr =
       let i = ctr in
       let ai = index a (i+a_idx) in 
       let bi = index b (i+b_idx) in 
-      gcut(fun _ -> v (get h0 a (i+a_idx)) + v (get h0 b (i+b_idx)) < pow2 platform_wide);
+      cut(v (get h0 a (i+a_idx)) + v (get h0 b (i+b_idx)) < pow2 platform_wide);
       let z = ai ^^+ bi in 
       upd a (a_idx+i) z; 
       let h1 = ST.get() in
       eq_lemma h0 h1 b (only a); 
       fsum_index a a_idx b b_idx len (ctr+1)
-      
-#reset-options
 
-abstract val gaddition_lemma: h0:heap -> h1:heap -> a:bigint_wide{live h0 a /\ live h1 a} -> b:bigint_wide{live h0 b} ->
-  len:nat{len <= length a /\ len <= length b /\ 
-	 (forall (i:nat). {:pattern (v (get h1 a i))} i < len ==> 
-	    v (get h1 a i) = v (get h0 a i) + v (get h0 b i)) } ->
-  GLemma unit (requires (True)) (ensures (eval h0 a len + eval h0 b len = eval h1 a len))
-let rec gaddition_lemma h0 h1 a b len =
-//  admit();
-  match len with
-  | 0 -> ()
-  | _ -> gaddition_lemma h0 h1 a b (len-1); 
-    distributivity_add_right (pow2 (bitweight templ (len-1))) (v (get h0 a (len-1)))  (v (get h0 b (len-1)))
-
-assume val addition_lemma: h0:heap -> h1:heap -> a:bigint_wide{live h0 a /\ live h1 a} -> b:bigint_wide{live h0 b} ->
+val addition_lemma: h0:heap -> h1:heap -> a:bigint_wide{live h0 a /\ live h1 a} -> b:bigint_wide{live h0 b} ->
   len:nat{len <= length a /\ len <= length b /\ 
 	 (forall (i:nat). {:pattern (v (get h1 a i))} i < len ==> 
 	    v (get h1 a i) = v (get h0 a i) + v (get h0 b i)) } ->
   Lemma (requires (True)) (ensures (eval h0 a len + eval h0 b len = eval h1 a len))
-(* let addition_lemma h0 h1 a b len = *)
-(*   coerce (requires (True)) (ensures (eval h0 a len + eval h0 b len = eval h1 a len)) *)
-(* 	 (fun _ -> gaddition_lemma h0 h1 a b len) *)
+let rec addition_lemma h0 h1 a b len =
+  match len with
+  | 0 -> ()
+  | _ -> addition_lemma h0 h1 a b (len-1); 
+    distributivity_add_right (pow2 (bitweight templ (len-1))) (v (get h0 a (len-1)))  (v (get h0 b (len-1)))
 
 let vmax = templ 0
 
@@ -83,7 +70,6 @@ val fsum': a:bigint_wide -> b:bigint_wide{disjoint a b} -> ST unit
       /\ isNotModified h0 h1 0 norm_length 0 a
       /\ isSum h0 h1 0 0 norm_length 0 a b))
 let fsum' a b =
-  admit();
   let h0 = ST.get() in 
   fsum_index a 0 b 0 norm_length 0; 
   let h1 = ST.get() in
